spc/IProp.v
@@ -2,6 +2,7 @@ Require Import Coqlib.
 Require Import String.
 Require Import PCM.
 Require Import Any.
+Require Import Program.
 
 Set Implicit Arguments.
 Set Typeclasses Depth 5.
